
\paragraph{Z Transforms}
\begin{center}
\large
\begin{tabular}{|c|c|}
\hline
\multicolumn{2}{|c|}{\textbf Table of Z Transforms}\\
\hline
$(x_k)_{k=0}^\infty$&  $Z \left[(x_k)_{k=0}^\infty \right]$\\
\hline
&\\
$x_k =\delta_k= \left\{ \begin{array}{ll} 1 & k = 0\\
   				 0 & k > 0
		\end{array} \right.$             & 1\\
(unit pulse)                 & \\
$x_k = r^k$ & $\frac{z}{z-r}$\\

$x_k = kr^{k-1}$ & $\frac{z}{(z-r)^2}$\\

\hline
\end{tabular}
\end{center}
{\textbf First shift theorem} (delaying):  if ${{Z}}[(x_k)]=X(z)$then
\[
{{Z}}[(x_{k-k_0})]=\frac{1}{z^{k_0}}X(z)
\]
where $x_k=0$for $k<0$.

\noindent {\textbf Second shift theorem} (advancing): if ${Z}[(x_k)]=X(z)$then
\[
{Z}[(x_{k+1})]=zX(z)-zx_0
\]
and
\[
{Z}[(x_{k+2})]=z^2X(z)-z^2x_0-zx_1
\]


\begin{table}[h]
	\begin{center}
	\begin{tabular}{c|c|c|c}
		\toprule 
		QUANTITY & SYMBOL & UNIT & UNIT ABBERVIATION 	\\
		Time & t & second & s				\\
		Frequency (cyclic) & f & hertz & Hz \\
		Frequency (radian) & $\omega $& radian/sec & rad/s	\\
		Phase angle &$\theta $, $\varphi $ & degree or radian & $^{\circ}$ or rad \\
		Energy & w & joule & J 	\\
		Power & p & watt & W	\\
		Charge & q  &coulomb & C	\\
		Current & i & ampere  &A	\\
		Electric field & E & volt/meter& V/m	\\
		Voltage & v & volt &V	\\
		Impedence & Z & ohm & $\varOmega$	\\
		Admittance &Y &siemen &S	\\
		Resistance &R &ohm &$\varOmega$	\\
		Conductance& G &siemen &S	\\
		Reactance &X &ohm &$\varOmega$	\\
		Susceptance &B &siemen& S	\\
		Inductance, self &L &henry& H	\\
		Inductance, mutual& M &henry& H	\\
		Capacitance& C& farad &F	\\
		Magnetic flux& $\phi$& weber &wb	\\
		Flux linkages& $\lambda$& weber-turns& wb-t	\\
		Power ratio& $log_{10}\frac{p_2}{p_1}$& Bel &B	\\
		\bottomrule
	\end{tabular}
	\caption{Electric Quantities}
\end{center}
\end{table}

 \begin{table}[h]
	
	\begin{center}
			\begin{tabular}{cccccc}
				\toprule 
				\multirow{1}{*}{}	& \multicolumn{2}{c}{\multirow{ 2}{*}{I-V RELATIONSHIPS}} &	\multicolumn{3}{c}{IMPENDENCE}  \\ \cline{4-6}
				& &	&  PHASOR-DOMAIN & s-DOMAIN & \\ \hline
				Resistor	& $v_R(t)=i_R(t) \times R=\dfrac{i_R(t)}{G}$& $i_R(t)=\dfrac{v_R(t)}{R}=v_R(t) \times G$& $ Z_R $ & R & R\\ \hline
				Inductor	& $v_L(t)=L\times \dfrac{ \partial i_L(t)}{\partial t} $& $i_L(t)=\dfrac{1}{L} \int_{0}^{t} v_L(x)dx+ i_L(0)$& $ Z_L $ &$ j\omega L$ & Ls\\ \hline
				Capacitor	& $v_C(t)=dfrac{1}{C}\int_{0}^{t} i_C(x)dx+ v_C(0)$& $i_C(t)=C\times \dfrac{\partial v_C(t)}{\partial t} $& $ Z_C $ & $ \dfrac{1}{j\omega C} $& $\dfrac{1}{Cs}$\\ 
				\bottomrule
			\end{tabular}
		\caption{Basic Circuit Relations}
	\end{center}
\end{table}


where 

\noindent{\textbf First shift theorem:} If $L(f(t))=F(s)$ then
$$ {\mathcal L}\left(e^{at}f(t)\right)=F(s-a).$$
{\textbf Third shift theorem:} If ${L}(f(t))=F(s)$ then
$$ {\mathcal L}\left(H_a(t)f(t-a)\right)=e^{-as}F(s).$$